Certify redo

src/lcertify/Certify.v
@@ -87,79 +87,215 @@ Proof.
 Qed.
 
 
-Inductive sim_time (ts:Time.t) (v1 v2:Time.t): Prop :=
+Inductive sim_time (ts:Time.t) (mem1 mem2:Memory.t) (v1 v2:Time.t): Prop :=
 | sim_time_intro
     (TS: v2 <= ts -> v1 = v2)
+    (WF1: v1 <= length mem1)
+    (WF2: v2 <= length mem2)
+    (ITF: forall loc (LAT: Memory.latest loc ts v2 mem2), Memory.latest loc ts v1 mem1)
 .
 Hint Constructors sim_time.
 
-Inductive sim_view (ts:Time.t) (v1 v2:View.t (A:=unit)): Prop :=
+Inductive sim_view (ts:Time.t) (mem1 mem2:Memory.t) (v1 v2:View.t (A:=unit)): Prop :=
 | sim_view_intro
     (TS: v2.(View.ts) <= ts -> v1 = v2)
+    (WF1: v1.(View.ts) <= length mem1)
+    (WF2: v2.(View.ts) <= length mem2)
+    (ITF: forall loc (LAT: Memory.latest loc ts v2.(View.ts) mem2), Memory.latest loc ts v1.(View.ts) mem1)
 .
 Hint Constructors sim_view.
 
-Inductive sim_val (ts:Time.t) (v1 v2:ValA.t (A:=View.t (A:=unit))): Prop :=
+Inductive sim_val (ts:Time.t) (mem1 mem2:Memory.t) (v1 v2:ValA.t (A:=View.t (A:=unit))): Prop :=
 | sim_val_intro
     (TS: v2.(ValA.annot).(View.ts) <= ts -> v1 = v2)
+    (WF1: v1.(ValA.annot).(View.ts) <= length mem1)
+    (WF2: v2.(ValA.annot).(View.ts) <= length mem2)
+    (ITF: forall loc (LAT: Memory.latest loc ts v2.(ValA.annot).(View.ts) mem2), Memory.latest loc ts v1.(ValA.annot).(View.ts) mem1)
 .
 Hint Constructors sim_val.
 
-Inductive sim_rmap (ts:Time.t) (rmap1 rmap2:RMap.t (A:=View.t (A:=unit))): Prop :=
+Inductive sim_rmap (ts:Time.t) (mem1 mem2:Memory.t) (rmap1 rmap2:RMap.t (A:=View.t (A:=unit))): Prop :=
 | sim_rmap_intro
-    (RMAP: IdMap.Forall2 (fun _ => sim_val ts) rmap1 rmap2)
+    (RMAP: IdMap.Forall2 (fun _ => sim_val ts mem1 mem2) rmap1 rmap2)
 .
 Hint Constructors sim_rmap.
 
-Inductive sim_state (ts:Time.t) (st1 st2:State.t (A:=View.t (A:=unit))): Prop :=
+Inductive sim_state (ts:Time.t) (mem1 mem2:Memory.t) (st1 st2:State.t (A:=View.t (A:=unit))): Prop :=
 | sim_state_intro
     (STMTS: st1.(State.stmts) = st2.(State.stmts))
-    (RMAP: sim_rmap ts st1.(State.rmap) st2.(State.rmap))
+    (RMAP: sim_rmap ts mem1 mem2 st1.(State.rmap) st2.(State.rmap))
 .
 Hint Constructors sim_state.
+
+Inductive sim_fwdbank (ts:Time.t) (mem1 mem2:Memory.t) (loc:Loc.t) (fwd1 fwd2:FwdItem.t (A:=unit)): Prop :=
+(* | sim_fwdbank_below *)
+(*     (TS2: fwd2.(FwdItem.ts) <= ts) *)
+(*     (VIEW2: fwd2.(FwdItem.view).(View.ts) <= fwd2.(FwdItem.ts)) *)
+(*     (EQ: fwd1 = fwd2) *)
+| sim_fwdbank_intro
+    val
+    (TS1: sim_time ts mem1 mem2 fwd1.(FwdItem.ts) fwd2.(FwdItem.ts))
+    (TS2: fwd2.(FwdItem.ts) > ts -> fwd1.(FwdItem.ts) > ts)
+    (VIEW: sim_view ts mem1 mem2 fwd1.(FwdItem.view) fwd2.(FwdItem.view))
+    (EX: fwd1.(FwdItem.ex) = fwd2.(FwdItem.ex))
+    (FWDTS1: fwd1.(FwdItem.view).(View.ts) <= fwd1.(FwdItem.ts))
+    (FWDTS2: fwd2.(FwdItem.view).(View.ts) <= fwd2.(FwdItem.ts))
+    (READ1: Memory.read loc fwd1.(FwdItem.ts) mem1 = Some val)
+    (READ2: Memory.read loc fwd2.(FwdItem.ts) mem2 = Some val)
+.
+
+(* TODO: move many lemmas *)
+(* TODO: move *)
+Ltac des_eq :=
+  repeat
+    (try match goal with
+         | [H: ?a === ?b |- _] => inv H
+         | [H: _ === riscv |- _] => revert H
+         | [H: proj_sumbool (equiv_dec ?a ?a) = true |- _] => clear H
+         | [H: proj_sumbool (equiv_dec ?a ?b) = _ |- _] => destruct (equiv_dec a b)
+         | [H: negb _ = true |- _] => apply Bool.negb_true_iff in H
+         | [H: negb _ = false |- _] => apply Bool.negb_false_iff in H
+         | [H: andb _ _ = false |- _] => apply Bool.andb_false_iff in H
+         | [H: andb _ _ = true |- _] => apply Bool.andb_true_iff in H
+         | [H: orb _ _ = false |- _] => apply Bool.orb_false_iff in H
+         end;
+     ss; des; subst; try congr).
+
+Lemma sim_fwd_view1 ts mem1 mem2 loc fwd1 fwd2 t o
+      (FWD: sim_fwdbank ts mem1 mem2 loc fwd1 fwd2)
+      (MEM1: ts <= length mem1)
+      (MEM2: ts <= length mem2)
+      (T: t <= ts)
+      (TS: fwd2.(FwdItem.ts) <= t):
+  sim_view ts mem1 mem2 (FwdItem.read_view fwd1 t o) (FwdItem.read_view fwd2 t o).
+Proof.
+  destruct fwd1 as [ts1 view1 ex1].
+  destruct fwd2 as [ts2 view2 ex2].
+  unfold FwdItem.read_view. s. inv FWD; ss; repeat condtac; ss.
+  all: repeat match goal with
+              | [H: sim_time _ _ _ _ _ |- _] => inv H
+              | [H: sim_view _ _ _ _ _ |- _] => inv H
+              end.
+  all: unfold Time.t in *.
+  all: des_eq.
+  all: try by econs; ss; ii; lia.
+  - econs; ss; ii; try lia.
+    rewrite TS0 in c; [|lia]. congr.
+  - econs; ss; ii; try lia.
+    rewrite TS0 in c; [|lia]. congr.
+  - econs; ss; ii; try lia.
+    rewrite TS0 in c; [|lia]. congr.
+  - econs; ss; ii; try lia.
+    rewrite TS0 in c; [|lia]. congr.
+Qed.
+
+(* TODO: move *)
+    Lemma latest_uniq
+          ts1 ts2 ts loc mem val1 val2
+          (TS1: ts1 <= ts)
+          (TS2: ts2 <= ts)
+          (LATEST1: Memory.latest loc ts1 ts mem)
+          (LATEST2: Memory.latest loc ts2 ts mem)
+          (MSG1: Memory.read loc ts1 mem = Some val1)
+          (MSG2: Memory.read loc ts2 mem = Some val2):
+      ts1 = ts2.
+    Proof.
+      destruct (Nat.lt_trichotomy ts1 ts2); des; ss.
+      - destruct ts2; [lia|]. exfalso.
+        revert MSG2. unfold Memory.read. s. destruct (nth_error mem ts2) eqn:NTH; ss.
+        condtac; ss. inversion e. subst. i. inv MSG2.
+        eapply LATEST1; eauto.
+      - destruct ts1; [lia|]. exfalso.
+        revert MSG1. unfold Memory.read. s. destruct (nth_error mem ts1) eqn:NTH; ss.
+        condtac; ss. inversion e. subst. i. inv MSG1.
+        eapply LATEST2; eauto.
+    Qed.
+
+Lemma sim_fwd_view2 ts mem1 mem2 loc fwd1 fwd2 ts1 ts2 o
+      (FWD: sim_fwdbank ts mem1 mem2 loc fwd1 fwd2)
+      (MEM1: ts <= length mem1)
+      (MEM2: ts <= length mem2)
+      (TS1: ts1 <= length mem1)
+      (TS2: ts2 <= length mem2)
+      (T1: ts1 <= ts)
+      (T2: ts2 > ts)
+      (FWDTS1: fwd1.(FwdItem.ts) <= ts1)
+      (FWDTS2: fwd2.(FwdItem.ts) <= ts2):
+  sim_view ts mem1 mem2 (FwdItem.read_view fwd1 ts1 o) (FwdItem.read_view fwd2 ts2 o).
+Proof.
+  destruct fwd1 as [tsf1 view1 ex1].
+  destruct fwd2 as [tsf2 view2 ex2].
+  unfold FwdItem.read_view in *. s. inv FWD; ss; repeat condtac; ss; subst.
+  all: repeat match goal with
+              | [H: sim_time _ _ _ _ _ |- _] => inv H
+              | [H: sim_view _ _ _ _ _ |- _] => inv H
+              end.
+  all: unfold Time.t in *.
+  all: des_eq.
+  all: try by econs; ss; ii; lia.
+Qed.
+
+      (* TODO: move *)
+      Lemma latest_mon
+            loc f t1 t2 mem
+            (LATEST: Memory.latest loc f t2 mem)
+            (T: t1 <= t2):
+        Memory.latest loc f t1 mem.
+      Proof.
+        ii. eapply LATEST; eauto. lia.
+      Qed.
+
+Lemma sim_fwd_view3 ts mem1 mem2 loc fwd1 fwd2 ts2 o
+      (FWD: sim_fwdbank ts mem1 mem2 loc fwd1 fwd2)
+      (MEM1: ts <= length mem1)
+      (MEM2: ts <= length mem2)
+      (TS2: ts2 <= length mem2)
+      (T2: ts2 > ts)
+      (FWDVIEW1: fwd1.(FwdItem.view).(View.ts) <= fwd1.(FwdItem.ts))
+      (FWDVIEW2: fwd2.(FwdItem.view).(View.ts) <= fwd2.(FwdItem.ts))
+      (FWDTS1: fwd1.(FwdItem.ts) <= length mem1)
+      (FWDTS2: fwd2.(FwdItem.ts) <= ts2):
+  sim_view ts mem1 mem2 (FwdItem.read_view fwd1 fwd1.(FwdItem.ts) o) (FwdItem.read_view fwd2 ts2 o).
+Proof.
+  destruct fwd1 as [tsf1 view1 ex1].
+  destruct fwd2 as [tsf2 view2 ex2].
+  unfold FwdItem.read_view in *. s. inv FWD; ss; repeat condtac; ss; subst.
+  all: repeat match goal with
+              | [H: sim_time _ _ _ _ _ |- _] => inv H
+              | [H: sim_view _ _ _ _ _ |- _] => inv H
+              end.
+  all: unfold Time.t in *.
+  all: des_eq.
+  all: try by econs; ss; ii; lia.
+  - econs; ss; i; try lia.
+    eapply ITF0. eapply latest_mon; eauto. lia.
+  - econs; ss; i; try lia.
+    eapply ITF0. eapply latest_mon; eauto. lia.
+  - econs; ss; i; try lia.
+    eapply ITF. eapply latest_mon; eauto.
+  - econs; ss; i; try lia.
+    eapply ITF. eapply latest_mon; eauto.
+Qed.
 
 Inductive sim_exbank (tid:Id.t) (ts:Time.t) (mem1 mem2:Memory.t) (eb1 eb2:Exbank.t (A:=unit)): Prop :=
 | sim_exbank_intro
     (LOC: eb1.(Exbank.loc) = eb2.(Exbank.loc))
-    (TS: sim_time ts eb1.(Exbank.ts) eb2.(Exbank.ts))
-    (EBVIEW: sim_view ts eb1.(Exbank.view) eb2.(Exbank.view))
+    (TS1: sim_time ts mem1 mem2 eb1.(Exbank.ts) eb2.(Exbank.ts))
+    (TS2: ts < eb2.(Exbank.ts) -> Memory.latest eb1.(Exbank.loc) ts eb1.(Exbank.ts) mem1)
+    (EBVIEW: sim_view ts mem1 mem2 eb1.(Exbank.view) eb2.(Exbank.view))
 .
+Hint Constructors sim_exbank.
 
-Inductive sim_fwdbank
-          (ts:Time.t) (loc:Loc.t) (coh1 coh2:Time.t)
-          (mem1 mem2:Memory.t)
-          (fwd1 fwd2:FwdItem.t (A:=unit)): Prop :=
-| sim_fwdbank_below
-    (TS2: fwd2.(FwdItem.ts) <= ts)
-    (FWD: fwd1 = fwd2)
-| sim_fwdbank_above
-    (TS1: fwd1.(FwdItem.ts) > ts)
-    (TS2: fwd2.(FwdItem.ts) > ts)
-    (VIEW2: fwd2.(FwdItem.view).(View.ts) > ts)
-| sim_fwdbank_mid
-    (TS1: fwd1.(FwdItem.ts) > ts)
-    (TS2: fwd2.(FwdItem.ts) > ts)
-    (VIEW2: fwd2.(FwdItem.view).(View.ts) <= ts)
-    (VIEW: fwd1.(FwdItem.view) = fwd2.(FwdItem.view))
-    (EX: fwd1.(FwdItem.ex) = fwd2.(FwdItem.ex))
-    (COH1: coh1 = fwd1.(FwdItem.ts))
-    (COH2: coh2 = fwd2.(FwdItem.ts))
-    (LATEST1: forall ts' val (READ: Memory.read loc ts' mem1 = Some val), ts' <= fwd1.(FwdItem.ts))
-    (LATEST2: forall ts' val (READ: Memory.read loc ts' mem2 = Some val), ts' <= fwd2.(FwdItem.ts))
-    (READ: Memory.read loc fwd1.(FwdItem.ts) mem1 = Memory.read loc fwd2.(FwdItem.ts) mem2)
-.
-
-Inductive sim_lc (tid:Id.t) (ts:Time.t) (lc1 lc2:Local.t (A:=unit)) (mem1 mem2:Memory.t): Prop :=
+Inductive sim_lc (tid:Id.t) (ts:Time.t) (mem1 mem2:Memory.t) (lc1 lc2:Local.t (A:=unit)): Prop :=
 | sim_lc_intro
-    (COH: forall loc, sim_time ts (lc1.(Local.coh) loc) (lc2.(Local.coh) loc))
-    (VRP: sim_view ts lc1.(Local.vrp) lc2.(Local.vrp))
-    (VWP: sim_view ts lc1.(Local.vwp) lc2.(Local.vwp))
-    (VRM: sim_view ts lc1.(Local.vrm) lc2.(Local.vrm))
-    (VWM: sim_view ts lc1.(Local.vwm) lc2.(Local.vwm))
-    (VCAP: sim_view ts lc1.(Local.vcap) lc2.(Local.vcap))
-    (VREL: sim_view ts lc1.(Local.vrel) lc2.(Local.vrel))
-    (FWDBANK: forall loc, sim_fwdbank ts loc (lc1.(Local.coh) loc) (lc2.(Local.coh) loc) mem1 mem2
-                                 (lc1.(Local.fwdbank) loc) (lc2.(Local.fwdbank) loc))
+    (COH: forall loc, sim_time ts mem1 mem2 (lc1.(Local.coh) loc) (lc2.(Local.coh) loc))
+    (VRP: sim_view ts mem1 mem2 lc1.(Local.vrp) lc2.(Local.vrp))
+    (VWP: sim_view ts mem1 mem2 lc1.(Local.vwp) lc2.(Local.vwp))
+    (VRM: sim_view ts mem1 mem2 lc1.(Local.vrm) lc2.(Local.vrm))
+    (VWM: sim_view ts mem1 mem2 lc1.(Local.vwm) lc2.(Local.vwm))
+    (VCAP: sim_view ts mem1 mem2 lc1.(Local.vcap) lc2.(Local.vcap))
+    (VREL: sim_view ts mem1 mem2 lc1.(Local.vrel) lc2.(Local.vrel))
+    (FWDBANK: forall loc, sim_fwdbank ts mem1 mem2 loc (lc1.(Local.fwdbank) loc) (lc2.(Local.fwdbank) loc))
     (EXBANK: opt_rel (sim_exbank tid ts mem1 mem2) lc1.(Local.exbank) lc2.(Local.exbank))
     (PROMISES1: forall tsp (TSP: tsp <= ts), Promises.lookup tsp lc1.(Local.promises) = Promises.lookup tsp lc2.(Local.promises))
     (PROMISES2: forall tsp (TSP: tsp > ts), Promises.lookup tsp lc1.(Local.promises) = false)
@@ -168,32 +304,44 @@ Hint Constructors sim_lc.
 
 Inductive sim_mem (tid:Id.t) (ts:Time.t) (mem1 mem2:Memory.t): Prop :=
 | sim_mem_intro
-    (EQUIV: forall tsx (TSX: tsx <= ts), Memory.get_msg tsx mem1 = Memory.get_msg tsx mem2)
+    mem mem1' mem2'
+    (MEM: ts = length mem)
+    (MEM1: mem1 = mem ++ mem1')
+    (MEM2: mem2 = mem ++ mem2')
+    (MEM1': List.Forall (fun msg => msg.(Msg.tid) = tid) mem1')
 .
 Hint Constructors sim_mem.
 
 Inductive sim_eu (tid:Id.t) (ts:Time.t) (eu1 eu2:ExecUnit.t (A:=unit)): Prop :=
 | sim_eu_intro
-    (STATE: sim_state ts eu1.(ExecUnit.state) eu2.(ExecUnit.state))
-    (LOCAL: sim_lc tid ts eu1.(ExecUnit.local) eu2.(ExecUnit.local) eu1.(ExecUnit.mem) eu2.(ExecUnit.mem))
+    (STATE: sim_state ts eu1.(ExecUnit.mem) eu2.(ExecUnit.mem) eu1.(ExecUnit.state) eu2.(ExecUnit.state))
+    (LOCAL: sim_lc tid ts eu1.(ExecUnit.mem) eu2.(ExecUnit.mem) eu1.(ExecUnit.local) eu2.(ExecUnit.local))
     (MEM: sim_mem tid ts eu1.(ExecUnit.mem) eu2.(ExecUnit.mem))
 .
 Hint Constructors sim_eu.
 
 Lemma sim_time_join
-      ts l1 l2 r1 r2
-      (VIEW1: sim_time ts l1 r1)
-      (VIEW2: sim_time ts l2 r2):
-  sim_time ts (join l1 l2) (join r1 r2).
+      ts mem1 mem2 l1 l2 r1 r2
+      (VIEW1: sim_time ts mem1 mem2 l1 r1)
+      (VIEW2: sim_time ts mem1 mem2 l2 r2):
+  sim_time ts mem1 mem2 (join l1 l2) (join r1 r2).
 Proof.
-  inv VIEW1. inv VIEW2.
-  econs. intro X. unfold join, Time.join in X. apply Time.max_lub_iff in X. des.
-  eauto.
+  inv VIEW1. inv VIEW2. econs.
+  - i. rewrite TS, TS0; ss.
+    + rewrite <- H, <- join_r. ss.
+    + rewrite <- H, <- join_l. ss.
+  - apply join_spec; ss.
+  - apply join_spec; ss.
+  - ii. apply Time.max_le in TS2. des.
+    + eapply ITF; eauto.
+      eapply latest_mon; eauto. apply join_l.
+    + eapply ITF0; eauto.
+      eapply latest_mon; eauto. apply join_r.
 Qed.
 
 Lemma sim_time_eq
-      ts v1 v2
-      (SIM: sim_time ts v1 v2)
+      ts mem1 mem2 v1 v2
+      (SIM: sim_time ts mem1 mem2 v1 v2)
       (V2: v2 <= ts):
   v1 = v2.
 Proof.
@@ -201,84 +349,107 @@ Proof.
 Qed.
 
 Lemma sim_val_const
-      ts c:
-  sim_val ts (ValA.mk _ c bot) (ValA.mk _ c bot).
+      ts mem1 mem2 c:
+  sim_val ts mem1 mem2 (ValA.mk _ c bot) (ValA.mk _ c bot).
 Proof.
-  econs. ss.
+  econs; splits; ss; try apply bot_spec.
+  ii. inv TS2.
 Qed.
 
 Lemma sim_view_bot
-      ts:
-  sim_view ts bot bot.
+      ts mem1 mem2:
+  sim_view ts mem1 mem2 bot bot.
 Proof.
-  econs. ss.
+  econs; splits; ss; try apply bot_spec.
+  ii. inv TS2.
 Qed.
 
 Lemma sim_view_const
-      ts c:
-  sim_view ts (View.mk c bot) (View.mk c bot).
+      ts mem1 mem2 c
+      (C1: c <= ts)
+      (C2: c <= length mem1)
+      (C3: c <= length mem2):
+  sim_view ts mem1 mem2 (View.mk c bot) (View.mk c bot).
 Proof.
-  econs. ss.
+  econs; ss. ii. lia.
 Qed.
 
 Lemma sim_view_join
-      ts l1 l2 r1 r2
-      (VIEW1: sim_view ts l1 r1)
-      (VIEW2: sim_view ts l2 r2):
-  sim_view ts (join l1 l2) (join r1 r2).
+      ts mem1 mem2 l1 l2 r1 r2
+      (VIEW1: sim_view ts mem1 mem2 l1 r1)
+      (VIEW2: sim_view ts mem1 mem2 l2 r2):
+  sim_view ts mem1 mem2 (join l1 l2) (join r1 r2).
 Proof.
   destruct l1 as [lt1 lv1].
   destruct l2 as [lt2 lv2].
   destruct r1 as [rt1 rv1].
   destruct r2 as [rt2 rv2].
-  inv VIEW1. inv VIEW2. ss.
-  econs. s. intro X. unfold join, Time.join in X. apply Time.max_lub_iff in X. des.
-  specialize (TS X). specialize (TS0 X0). des. inv TS. inv TS0. ss.
+  inv VIEW1. inv VIEW2. econs; ss.
+  - i. rewrite TS, TS0; ss.
+    + rewrite <- H, <- join_r. ss.
+    + rewrite <- H, <- join_l. ss.
+  - apply join_spec; ss.
+  - apply join_spec; ss.
+  - ii. apply Time.max_le in TS2. des.
+    + eapply ITF; eauto.
+      eapply latest_mon; eauto. apply join_l.
+    + eapply ITF0; eauto.
+      eapply latest_mon; eauto. apply join_r.
 Qed.
 
 Lemma sim_view_ifc
-      ts c l1 r1
-      (VIEW1: sim_view ts l1 r1):
-  sim_view ts (ifc c l1) (ifc c r1).
+      ts mem1 mem2 c l1 r1
+      (VIEW1: sim_view ts mem1 mem2 l1 r1):
+  sim_view ts mem1 mem2 (ifc c l1) (ifc c r1).
 Proof.
-  destruct c; ss.
+  destruct c; ss. apply sim_view_bot.
 Qed.
 
 Lemma sim_view_eq
-      ts v1 v2
-      (SIM: sim_view ts v1 v2)
+      ts mem1 mem2 v1 v2
+      (SIM: sim_view ts mem1 mem2 v1 v2)
       (V2: v2.(View.ts) <= ts):
   v1 = v2.
 Proof.
   apply SIM. ss.
 Qed.
 
-Lemma sim_val_view ts v1 v2
-      (VAL: sim_val ts v1 v2):
-  sim_view ts v1.(ValA.annot) v2.(ValA.annot).
+Lemma sim_val_view ts mem1 mem2 v1 v2
+      (VAL: sim_val ts mem1 mem2 v1 v2):
+  sim_view ts mem1 mem2 v1.(ValA.annot) v2.(ValA.annot).
 Proof.
-  inv VAL. econs. i. specialize (TS H). des. subst. ss.
+  inv VAL. econs; ss. i. rewrite TS; ss.
 Qed.
 
 Lemma sim_rmap_expr
-      ts rmap1 rmap2 e
-      (RMAP: sim_rmap ts rmap1 rmap2):
-  sim_val ts (sem_expr rmap1 e) (sem_expr rmap2 e).
+      ts mem1 mem2 rmap1 rmap2 e
+      (RMAP: sim_rmap ts mem1 mem2 rmap1 rmap2):
+  sim_val ts mem1 mem2 (sem_expr rmap1 e) (sem_expr rmap2 e).
 Proof.
   induction e; s.
   - apply sim_val_const.
   - unfold RMap.find. inv RMAP. specialize (RMAP0 reg). inv RMAP0; ss.
-  - econs. s. i. inv IHe. specialize (TS H). des. congr.
-  - econs. s. i. unfold join, Time.join in H. apply Time.max_lub_iff in H. des.
-    inv IHe1. inv IHe2.
-    specialize (TS H). specialize (TS0 H0). des. congr.
+    apply sim_val_const.
+  - inv IHe. econs; ss.
+    i. rewrite TS; ss.
+  - inv IHe1. inv IHe2. econs; ss.
+    + i. rewrite TS, TS0; ss.
+      * rewrite <- H, <- join_r. ss.
+      * rewrite <- H, <- join_l. ss.
+    + apply join_spec; ss.
+    + apply join_spec; ss.
+    + ii. apply Time.max_le in TS2. des.
+      * eapply ITF; eauto.
+        eapply latest_mon; eauto. apply join_l.
+      * eapply ITF0; eauto.
+        eapply latest_mon; eauto. apply join_r.
 Qed.
 
 Lemma sim_rmap_add
-      ts rmap1 rmap2 v1 v2 r
-      (RMAP: sim_rmap ts rmap1 rmap2)
-      (VAL: sim_val ts v1 v2):
-  sim_rmap ts (RMap.add r v1 rmap1) (RMap.add r v2 rmap2).
+      ts mem1 mem2 rmap1 rmap2 v1 v2 r
+      (RMAP: sim_rmap ts mem1 mem2 rmap1 rmap2)
+      (VAL: sim_val ts mem1 mem2 v1 v2):
+  sim_rmap ts mem1 mem2 (RMap.add r v1 rmap1) (RMap.add r v2 rmap2).
 Proof.
   inv RMAP. econs. ii. unfold RMap.add. rewrite ? IdMap.add_spec.
   condtac; ss. inversion e. subst. econs. ss.
@@ -290,67 +461,32 @@ Lemma sim_mem_read
       (TS0: ts0 <= ts):
   Memory.read loc ts0 mem1 = Memory.read loc ts0 mem2.
 Proof.
-  inv SIM. generalize (EQUIV _ TS0). unfold Memory.get_msg, Memory.read. destruct ts0; ss.
-  intro X. rewrite X. ss.
+  inv SIM. unfold Memory.read. destruct ts0; ss. rewrite ? nth_error_app1; ss.
+Qed.
+
+Lemma sim_mem_get_msg
+      tid ts mem1 mem2 ts0
+      (SIM: sim_mem tid ts mem1 mem2)
+      (TS0: ts0 <= ts):
+  Memory.get_msg ts0 mem1 = Memory.get_msg ts0 mem2.
+Proof.
+  inv SIM. unfold Memory.get_msg. destruct ts0; ss. rewrite ? nth_error_app1; ss.
+Qed.
+
+Lemma sim_mem_length
+      tid ts mem1 mem2
+      (SIM: sim_mem tid ts mem1 mem2):
+  ts <= length mem1 /\ ts <= length mem2.
+Proof.
+  inv SIM. rewrite ? List.app_length. splits; lia.
 Qed.
 
 Lemma sim_view_val
-      ts c v1 v2
-      (SIM: sim_view ts v1 v2):
-  sim_val ts (ValA.mk _ c v1) (ValA.mk _ c v2).
+      ts mem1 mem2 c v1 v2
+      (SIM: sim_view ts mem1 mem2 v1 v2):
+  sim_val ts mem1 mem2 (ValA.mk _ c v1) (ValA.mk _ c v2).
 Proof.
-  inv SIM. econs. s. i. rewrite TS; ss.
-Qed.
-
-(* TODO: move *)
-Ltac des_eq :=
-  repeat
-    (try match goal with
-         | [H: context[equiv_dec ?a ?b] |- _] => destruct (equiv_dec a b)
-         | [H: _ === riscv |- _] => revert H
-         | [H: ?a === ?b |- _] => inv H
-         | [H: negb _ = true |- _] => apply Bool.negb_true_iff in H
-         | [H: negb _ = false |- _] => apply Bool.negb_false_iff in H
-         | [H: andb _ _ = false |- _] => apply Bool.andb_false_iff in H
-         | [H: andb _ _ = true |- _] => apply Bool.andb_true_iff in H
-         end;
-     ss; des; subst; try congr).
-
-Lemma sim_fwd_view1 ts loc lc1 lc2 mem1 mem2 fwd1 fwd2 t o
-      (FWD: sim_fwdbank ts loc lc1 lc2 mem1 mem2 fwd1 fwd2)
-      (T: t <= ts):
-  sim_view ts (FwdItem.read_view fwd1 t o) (FwdItem.read_view fwd2 t o).
-Proof.
-  destruct fwd1 as [ts1 view1 ex1].
-  destruct fwd2 as [ts2 view2 ex2].
-  unfold FwdItem.read_view. s. inv FWD; ss; repeat condtac; ss.
-  all: try inv FWD0.
-  all: des_eq.
-  all: try by econs; ss; lia.
-Qed.
-
-Lemma sim_fwd_view2 ts loc lc1 lc2 mem1 mem2 fwd1 fwd2 ts2 o
-      (FWD: sim_fwdbank ts loc lc1 lc2 mem1 mem2 fwd1 fwd2)
-      (T2: ts2 > ts)
-      (VIEW2: (fwd2.(FwdItem.read_view) ts2 o).(View.ts) <= ts):
-  <<TS1: fwd1.(FwdItem.ts) > ts>> /\
-  <<TS2: fwd2.(FwdItem.ts) = ts2>> /\
-  <<VIEW1: sim_view ts (FwdItem.read_view fwd1 fwd1.(FwdItem.ts) o) (FwdItem.read_view fwd2 fwd2.(FwdItem.ts) o)>> /\
-  <<VIEW2: fwd1.(FwdItem.view) = fwd2.(FwdItem.view)>> /\
-  <<VIEW3: fwd2.(FwdItem.view).(View.ts) <= ts>> /\
-  <<EX: fwd1.(FwdItem.ex) = fwd2.(FwdItem.ex)>> /\
-  <<COH1: lc1 = fwd1.(FwdItem.ts)>> /\
-  <<COH2: lc2 = fwd2.(FwdItem.ts)>> /\
-  <<LATEST1: forall ts' val (READ: Memory.read loc ts' mem1 = Some val), ts' <= fwd1.(FwdItem.ts)>> /\
-  <<LATEST2: forall ts' val (READ: Memory.read loc ts' mem2 = Some val), ts' <= fwd2.(FwdItem.ts)>> /\
-  <<READ: Memory.read loc fwd1.(FwdItem.ts) mem1 = Memory.read loc fwd2.(FwdItem.ts) mem2>>.
-Proof.
-  destruct fwd1 as [tsf1 view1 ex1].
-  destruct fwd2 as [tsf2 view2 ex2].
-  unfold FwdItem.read_view in *. s. revert VIEW2. inv FWD; ss; repeat condtac; ss.
-  all: try inv FWD0.
-  all: des_eq. 
-  all: try by econs; splits; ss; lia.
+  inv SIM. econs; ss. i. rewrite TS; ss.
 Qed.
 
 Lemma sim_eu_step
@@ -400,8 +536,12 @@ Proof.
       intro ELOC. rewrite ELOC in *. clear TS.
       inv LOCAL.
       destruct (le_lt_dec ts0 ts).
-      { (* tgt read <= ts. *)
-        exploit sim_fwd_view1; eauto. intro FWDVIEW.
+      { (* Case 1: tgt read <= ts. *)
+        exploit sim_fwd_view1; eauto.
+        { exploit sim_mem_length; eauto. i. des. ss. }
+        { exploit sim_mem_length; eauto. i. des. ss. }
+        { rewrite <- COH. apply WF2. }
+        intro FWDVIEW.
         eexists (ExecUnit.mk _ _ _). esplits.
         - econs 1. econs. econs; ss.
           + econs; ss.
@@ -413,60 +553,65 @@ Proof.
             * admit. (* Memory.read *)
         - econs; ss.
           + econs; ss. apply sim_rmap_add; ss. apply sim_view_val.
-            rewrite POST. eauto 10 using sim_view_join, sim_view_ifc.
-          + econs; ss; try by rewrite ? POST; eauto 10 using sim_view_join, sim_view_ifc.
-            * i. rewrite ? fun_add_spec. condtac; ss.
-            * i. rewrite ? fun_add_spec. condtac; ss. inversion e. subst.
-              admit. (* sim_fwdbank *)
-            * destruct ex0; ss. econs. econs; ss. rewrite POST. eauto 10 using sim_view_join, sim_view_ifc.
+            rewrite POST. eauto 10 using sim_view_join, sim_view_ifc, sim_view_bot.
+          + econs; ss; try by rewrite ? POST; eauto 10 using sim_view_join, sim_view_ifc, sim_view_bot.
+            * i. rewrite ? fun_add_spec. condtac; ss. admit. (* easy *)
+            * destruct ex0; ss. econs. econs; ss.
+              { admit. (* easy *) }
+              { i. admit. (* WRONG : TODO *) }
+              { rewrite POST. eauto 10 using sim_view_join, sim_view_ifc, sim_view_bot. }
       }
-      (* tgt read > ts. *)
+      (* Case 2: tgt read > ts. *)
       destruct (le_lt_dec post.(View.ts) ts).
       { (* if post-view <= ts, then read should be forwarded. *)
-        rename l0 into POST'.
-        exploit sim_fwd_view2; eauto.
-        { rewrite <- POST', POST. s. rewrite <- join_r. refl. }
-        i. des. subst.
-        eexists (ExecUnit.mk _ _ _). esplits.
-        - econs 1. econs. econs; ss.
-          + econs; ss.
-          + rewrite ELOC in *.
-            econs 2; eauto. instantiate (2 := (FwdItem.ts (Local.fwdbank lc1 (ValA.val (sem_expr rmap2 eloc))))). econs; ss.
-            * rewrite COH1. ss.
-            * admit. (* Memory.latest *)
-            * rewrite READ, MSG. ss.
-        - econs; ss.
-          + econs; ss. apply sim_rmap_add; ss. apply sim_view_val.
-            rewrite POST. eauto 10 using sim_view_join, sim_view_ifc.
-          + econs; ss; try by rewrite ? POST; eauto 10 using sim_view_join, sim_view_ifc.
-            * i. rewrite ? fun_add_spec. condtac; ss. econs. lia.
-            * i. rewrite ? fun_add_spec. condtac; ss. inversion e. subst. econs 3; ss.
-            * destruct ex0; ss. econs. econs; ss.
-              { econs. lia. }
-              { rewrite POST. eauto 10 using sim_view_join, sim_view_ifc. }
+        admit.
+        (* rename l0 into POST'. *)
+        (* exploit sim_fwd_view2; eauto. *)
+        (* { exploit sim_mem_length; eauto. i. des. ss. } *)
+        (* { exploit sim_mem_length; eauto. i. des. ss. } *)
+        (* { rewrite <- POST', POST. s. rewrite <- join_l, <- join_l. refl. } *)
+        (* i. des. subst. *)
+        (* eexists (ExecUnit.mk _ _ _). esplits. *)
+        (* - econs 1. econs. econs; ss. *)
+        (*   + econs; ss. *)
+        (*   + rewrite ELOC in *. *)
+        (*     econs 2; eauto. instantiate (2 := (FwdItem.ts (Local.fwdbank lc1 (ValA.val (sem_expr rmap2 eloc))))). econs; ss. *)
+        (*     * rewrite COH1. ss. *)
+        (*     * admit. (* Memory.latest *) *)
+        (*     * rewrite READ, MSG. ss. *)
+        (* - econs; ss. *)
+        (*   + econs; ss. apply sim_rmap_add; ss. apply sim_view_val. *)
+        (*     rewrite POST. eauto 10 using sim_view_join, sim_view_ifc. *)
+        (*   + econs; ss; try by rewrite ? POST; eauto 10 using sim_view_join, sim_view_ifc. *)
+        (*     * i. rewrite ? fun_add_spec. condtac; ss. econs. lia. *)
+        (*     * i. rewrite ? fun_add_spec. condtac; ss. inversion e. subst. econs 3; ss. *)
+        (*     * destruct ex0; ss. econs. econs; ss. *)
+        (*       { econs. lia. } *)
+        (*       { rewrite POST. eauto 10 using sim_view_join, sim_view_ifc. } *)
       }
       { (* if post-view > ts, then read the latest message. *)
-        exploit Memory.get_latest; eauto. i. des.
-        eexists (ExecUnit.mk _ _ _). esplits.
-        - econs 1. econs. econs; ss.
-          + econs; ss.
-          + rewrite ELOC in *.
-            econs 2; eauto. instantiate (2 := ts1). econs; ss.
-            * admit. (* coh <= ts1 *)
-            * admit. (* Memory.latest *)
-            * eauto.
-        - econs; ss.
-          + econs; ss. apply sim_rmap_add; ss. econs. s. lia.
-          + econs; ss; try by rewrite ? POST; eauto 10 using sim_view_join, sim_view_ifc.
-            * i. rewrite ? fun_add_spec. condtac; ss. inversion e. subst. econs. lia.
-            * apply sim_view_join; ss. unfold ifc. condtac; ss. econs. lia.
-            * apply sim_view_join; ss. unfold ifc. condtac; ss. econs. lia.
-            * apply sim_view_join; ss. econs. lia.
-            * i. rewrite ? fun_add_spec. condtac; ss. inversion e. subst.
-              admit. (* sim fwdbank *)
-            * destruct ex0; ss. econs. econs; ss.
-              { econs. lia. }
-              { econs. lia. }
+        admit.
+        (* exploit Memory.get_latest; eauto. i. des. *)
+        (* eexists (ExecUnit.mk _ _ _). esplits. *)
+        (* - econs 1. econs. econs; ss. *)
+        (*   + econs; ss. *)
+        (*   + rewrite ELOC in *. *)
+        (*     econs 2; eauto. instantiate (2 := ts1). econs; ss. *)
+        (*     * admit. (* coh <= ts1 *) *)
+        (*     * admit. (* Memory.latest *) *)
+        (*     * eauto. *)
+        (* - econs; ss. *)
+        (*   + econs; ss. apply sim_rmap_add; ss. econs. s. lia. *)
+        (*   + econs; ss; try by rewrite ? POST; eauto 10 using sim_view_join, sim_view_ifc. *)
+        (*     * i. rewrite ? fun_add_spec. condtac; ss. inversion e. subst. econs. lia. *)
+        (*     * apply sim_view_join; ss. unfold ifc. condtac; ss. econs. lia. *)
+        (*     * apply sim_view_join; ss. unfold ifc. condtac; ss. econs. lia. *)
+        (*     * apply sim_view_join; ss. econs. lia. *)
+        (*     * i. rewrite ? fun_add_spec. condtac; ss. inversion e. subst. *)
+        (*       admit. (* sim fwdbank *) *)
+        (*     * destruct ex0; ss. econs. econs; ss. *)
+        (*       { econs. lia. } *)
+        (*       { econs. lia. } *)
       }
     - (* fulfill *)
       inv STEP.
@@ -486,7 +631,7 @@ Proof.
         eexists (ExecUnit.mk _ _ _). esplits.
         + econs 1. econs. econs; ss; cycle 1.
           * econs 3; eauto. econs; eauto; cycle 1.
-            { rewrite <- MSG. apply MEM. ss. }
+            { rewrite <- MSG. eapply sim_mem_get_msg; eauto. }
             { inv LOCAL. rewrite PROMISES1; ss. }
             { instantiate (1 := view_ext).
               instantiate (1 := ord).
@@ -496,8 +641,9 @@ Proof.
                 { etrans; [by apply Time.lt_le_incl; eauto|]. eauto. }
                 s. repeat apply sim_view_join; ss.
                 all: try apply sim_view_ifc.
+                all: try apply sim_view_bot.
                 all: try by apply LOCAL.
-                inv LOCAL. inv EXBANK; ss. inv REL. ss.
+                all: admit.
               - exploit sim_time_eq.
                 { inv LOCAL. eapply COH0. }
                 { etrans; [by apply Time.lt_le_incl; eauto|]. eauto. }
@@ -506,23 +652,30 @@ Proof.
                 destruct a, eb. inv REL. ss. subst.
                 esplits; eauto. s. ii. subst.
                 inv WF2. ss. inv LOCAL. exploit EXBANK; eauto. s. i. des.
-                destruct (le_lt_dec ts2 ts).
-                { inv TS. specialize (TS3 l). subst.
-                  eapply EX0; eauto. rewrite <- MSG0. inv MEM.
-                  exploit (EQUIV (S ts3)).
-                  { lia. }
-                  unfold Memory.get_msg, Memory.read. ss.
-                }
-                { lia. }
+                admit.
+                (* destruct (le_lt_dec ts2 ts). *)
+                (* { inv TS. specialize (TS3 l). subst. *)
+                (*   eapply EX0; eauto. rewrite <- MSG0. inv MEM. *)
+                (*   exploit (EQUIV (S ts3)). *)
+                (*   { lia. } *)
+                (*   unfold Memory.get_msg, Memory.read. ss. *)
+                (* } *)
+                (* { lia. } *)
             }
           * econs 4; ss.
-        + econs; ss; eauto using sim_rmap_add, sim_val_const.
+        + econs; ss.
+          { econs; ss. apply sim_rmap_add; ss.
+            admit.
+          }
           inv LOCAL. econs; ss; i.
           all: repeat rewrite fun_add_spec.
           all: repeat apply sim_view_join; ss.
-          * condtac; ss.
-          * condtac; ss. inversion e. subst. econs 1; ss.
-          * destruct ex0; ss.
+          all: try condtac; ss.
+          * admit. (* easy *)
+          * admit. (* easy *)
+          * admit.
+          * admit.
+          * admit.
           * rewrite ? Promises.unset_o. condtac; ss. eauto.
           * rewrite Promises.unset_o. condtac; ss. eauto.
       }
@@ -547,7 +700,7 @@ Proof.
       + econs 1. econs. econs; ss; cycle 1.
         * econs 6; eauto. econs; eauto.
         * econs 5.
-      + econs; ss. inv LOCAL. econs; eauto 10 using sim_view_join, sim_view_ifc.
+      + econs; ss. inv LOCAL. econs; eauto 10 using sim_view_join, sim_view_ifc, sim_view_bot.
     - (* if *)
       inv LC. eexists (ExecUnit.mk _ _ _). esplits.
       + econs 1. econs. econs; ss; cycle 1.
@@ -559,7 +712,7 @@ Proof.
         { econs; ss. rewrite ELOC. ss. }
         econs; ss; try by apply LOCAL.
         apply sim_view_join; try by apply LOCAL.
-        rewrite ELOC. econs. ss.
+        rewrite ELOC. admit. (* sim_view refl *)
     - (* dowhile *)
       eexists (ExecUnit.mk _ _ _). esplits.
       + econs 1. econs. econs; ss; cycle 1.
@@ -569,10 +722,118 @@ Proof.
   }
 Admitted.
 
-Lemma sim_certify
-      tid eu1 eu2
-      (STATE: True)
-      (CERTIFY: certify tid eu1):
-  certify tid eu2.
+Lemma sim_eu_promises
+      tid ts eu1 eu2
+      (SIM: sim_eu tid ts eu1 eu2)
+      (EU2: forall tsp (TSP: tsp <= ts), Promises.lookup tsp eu2.(ExecUnit.local).(Local.promises) = false):
+  eu1.(ExecUnit.local).(Local.promises) = bot.
 Proof.
+  apply Promises.ext. i. rewrite Promises.lookup_bot.
+  inv SIM. inv LOCAL. destruct (le_dec i ts).
+  - rewrite PROMISES1, EU2; ss.
+  - rewrite PROMISES2; ss. lia.
+Qed.
+
+Lemma sim_eu_rtc_step
+      tid ts eu1 eu2 eu2'
+      (SIM: sim_eu tid ts eu1 eu2)
+      (STEP: rtc (certify_step tid) eu2 eu2')
+      (WF1: ExecUnit.wf tid eu1)
+      (WF2: ExecUnit.wf tid eu2)
+      (PROMISES: eu2'.(ExecUnit.local).(Local.promises) = bot):
+  exists eu1',
+    <<STEP: rtc (certify_step tid) eu1 eu1'>> /\
+    <<PROMISES: eu1'.(ExecUnit.local).(Local.promises) = bot>>.
+Proof.
+  revert eu1 SIM WF1 WF2. induction STEP; ss.
+  { esplits; eauto.
+    eapply sim_eu_promises; eauto. rewrite PROMISES.
+    i. rewrite Promises.lookup_bot. ss.
+  }
+  i. destruct (le_lt_dec (View.ts (Local.vcap (ExecUnit.local y))) ts).
+  - exploit sim_eu_step; eauto. i. des.
+    exploit certify_step_wf; try exact H; eauto. i.
+    exploit certify_step_wf; eauto. i.
+    exploit IHSTEP; eauto. i. des.
+    esplits; [|by eauto]. econs; eauto.
+  - esplits; eauto. eapply sim_eu_promises; eauto. i.
+    assert (PROMISES': forall tsp (TSP: tsp <= ts), Promises.lookup tsp y.(ExecUnit.local).(Local.promises) = false).
+    { admit. }
+    destruct x as [st1 lc1 mem1].
+    destruct y as [st2 lc2 mem2].
+    ss. inv H.
+    + inv STEP0. inv STEP1. ss. subst.
+      inv STATE; inv LOCAL; inv EVENT; ss.
+      all: eauto.
+      all: try inv STEP0; ss; eauto.
+      all: try inv LC; ss; eauto.
+      generalize (PROMISES' tsp TSP). rewrite Promises.unset_o. condtac; ss. inversion e. subst.
+      inv WRITABLE. ss. admit. (* easy *)
+    + inv STEP0. ss. admit. (* quite the same *)
+Admitted.
+
+Lemma state_step_certify
+      tid eu1 eu2
+      (CERTIFY: certify tid eu2)
+      (STEP: ExecUnit.state_step tid eu1 eu2):
+  certify tid eu1.
+Proof.
+  inv CERTIFY. econs; [|by eauto]. econs; eauto.
+Qed.
+
+Lemma promise_step_certify
+      tid eu1 eu2
+      (CERTIFY: certify tid eu2)
+      (STEP: ExecUnit.promise_step tid eu1 eu2)
+      (WF: ExecUnit.wf tid eu1):
+  certify tid eu1.
+Proof.
+  destruct (classic (eu1.(ExecUnit.local).(Local.promises) = bot)).
+  { econs; eauto. }
+  rename H into PROMISES.
+
+  assert (SIM: sim_eu tid (length eu1.(ExecUnit.mem)) eu1 eu2).
+  { destruct eu1 as [st1 lc1 mem1].
+    destruct eu2 as [st2 lc2 mem2].
+    inv STEP. inv LOCAL. ss. subst. inv MEM2. subst. econs; ss.
+    - econs; ss. econs. ii.
+      destruct (IdMap.find id (State.rmap st2)) eqn:FIND; ss. econs.
+      inv WF. ss. inv STATE. exploit RMAP; eauto. unfold RMap.find. rewrite FIND. i.
+      econs; ss.
+      + rewrite List.app_length. s. lia.
+      + ii. eapply LAT; eauto. apply nth_error_app_mon. ss.
+    - admit. (* sim_lc; easy *)
+    - econs; ss. rewrite app_nil_r. ss.
+  }
+
+  inv CERTIFY. exploit sim_eu_rtc_step; eauto.
+  { eapply ExecUnit.promise_step_wf; eauto. }
+  i. des. econs; eauto.
+Admitted.
+
+Lemma interference_certify
+      tid st lc mem mem_interference
+      (CERTIFY: certify tid (ExecUnit.mk st lc (mem ++ mem_interference)))
+      (WF: ExecUnit.wf tid (ExecUnit.mk st lc mem)):
+  certify tid (ExecUnit.mk st lc mem).
+Proof.
+  destruct (classic (lc.(Local.promises) = bot)).
+  { econs; eauto. }
+  rename H into PROMISES.
+
+  assert (SIM: sim_eu tid (length mem) (ExecUnit.mk st lc mem) (ExecUnit.mk st lc (mem ++ mem_interference))).
+  { econs; ss.
+    - econs; ss. econs. ii.
+      destruct (IdMap.find id (State.rmap st)) eqn:FIND; ss. econs.
+      inv WF. ss. inv STATE. exploit RMAP; eauto. unfold RMap.find. rewrite FIND. i.
+      econs; ss.
+      + rewrite List.app_length. s. lia.
+      + ii. eapply LAT; eauto. apply nth_error_app_mon. ss.
+    - admit. (* sim_lc; easy *)
+    - econs; ss. rewrite app_nil_r. ss.
+  }
+
+  inv CERTIFY. exploit sim_eu_rtc_step; eauto.
+  { admit. (* wf preserved *) }
+  i. des. econs; eauto.
 Admitted.
